cslib/Cslib.lean
@@ -54,6 +54,7 @@ public import Cslib.Computability.Languages.OmegaLanguage
 public import Cslib.Computability.Languages.OmegaRegularLanguage
 public import Cslib.Computability.Languages.RegularLanguage
 public import Cslib.Computability.Languages.SafetyLiveness
+public import Cslib.Computability.Machines.Turing.MultiTape.ConfigBound
 public import Cslib.Computability.Machines.Turing.MultiTape.Configuration
 public import Cslib.Computability.Machines.Turing.MultiTape.Deterministic
 public import Cslib.Computability.Machines.Turing.MultiTape.DeterministicToNondeterministic
